src/OPred.v
@@ -1,0 +1,109 @@
+(*===========================================================================
+    Predicates over observations
+  ===========================================================================*)
+Require Import ssreflect ssrfun ssrbool eqtype fintype finfun seq tuple.
+Require Import bitsrep ioaction ilogic.
+Require Import Setoid CSetoid RelationClasses Morphisms.
+
+Set Implicit Arguments.
+Unset Strict Implicit.
+Import Prenex Implicits.
+
+Local Obligation Tactic := idtac.
+
+Instance OEquiv : Equiv Obs := {
+   equiv o1 o2 := o1 = o2
+}.
+
+Instance OType : type Obs.
+Proof.
+  split.
+  move => x; by reflexivity.
+  move => x y H; by symmetry. 
+  move => x y z H1 H2; by rewrite H1 H2. 
+Qed.
+
+
+Definition OPred := ILFunFrm Obs Prop. 
+
+Local Existing Instance ILFun_Ops.
+Local Existing Instance ILFun_ILogic.
+
+Instance OLogicOps : ILogicOps OPred := _.
+Instance OLogic : ILogic OPred := _. 
+
+Implicit Arguments mkILFunFrm [[e] [ILOps]].
+
+Definition mkOPred (P : Obs -> Prop) 
+        (f : forall t t', t === t' -> P t |-- P t') : OPred :=
+  mkILFunFrm (seq (Chan*Data)) Prop P f.
+
+Implicit Arguments mkOPred [].
+
+Program Definition eq_opred s := mkOPred (fun s' => s === s') _.
+Next Obligation. move => s t t' EQ. by rewrite EQ. Qed.
+
+Program Definition catOP (P Q: OPred) : OPred
+ := @mkILFunFrm Obs _ Prop _ (fun o => exists o1 o2, o = o1++o2 /\ P o1 /\ Q o2) _.
+Next Obligation.
+move => P Q o o' EQ [o1 [o2 [H1 [H2 H3]]]]. 
+exists o1, o2. by subst.
+Qed.
+
+Program Definition empOP : OPred :=   
+  mkILFunFrm _ _ (fun o => o = nil) _.
+Next Obligation.
+move => o o' EQ. by setoid_rewrite EQ. 
+Qed. 
+
+Local Transparent ILFun_Ops ILPre_Ops.
+
+Instance catOP_entails_m: Proper (lentails ==> lentails ==> lentails) catOP.
+Proof.
+move => O1 O1' HO1 O2 O2' HO2. move => s/= H. 
+destruct H as [o1 [o2 [H1 [H2 H3]]]]. subst. 
+exists o1, o2. split => //. split. by apply HO1. by apply HO2. 
+Qed. 
+
+Instance catSP_lequiv_m: Proper (lequiv ==> lequiv ==> lequiv) catOP.
+Proof.
+  intros P P' HP Q Q' HQ.
+  split; apply catOP_entails_m; (apply HP || apply HQ).
+Qed.
+
+
+Definition outOP (c:Chan) (d:Data) : OPred := eq_opred [::(c,d)]. 
+Definition seqOP (o:Obs) : OPred := eq_opred o.
+
+Lemma empOPR P : catOP P empOP -|- P.
+Proof.
+split.
+move => o [s1 [s2 [H1 [H2 /=H3]]]]. subst. by rewrite cats0. 
+move => o H. simpl. exists o, nil. by rewrite cats0. 
+Qed. 
+
+Lemma empOPL P : catOP empOP P -|- P.
+Proof.
+split.
+move => o [s1 [s2 [H1 [/=H2 H3]]]]. by subst. 
+move => o H. simpl. by exists nil, o. 
+Qed.
+
+Lemma catOPA (P Q R : OPred) : catOP (catOP P Q) R -|- catOP P (catOP Q R).
+Proof.
+split. 
++ move => o [s1 [s2 [H1 [[s3 [s4 [H2 [H3 H4]]]] H5]]]]. subst. simpl.
+  exists s3, (s4++s2). rewrite catA. split => //. split => //. by exists s4, s2. 
++ move => o [s1 [s2 [H1 [H2 [s3 [s4 [H3 [H4 H5]]]]]]]]. subst. simpl. 
+  exists (s1++s3), s4. rewrite catA. split => //. split => //. by exists s1, s3. 
+Qed. 
+
+Lemma land_catOP P Q R : catOP (P//\\Q) R |-- (catOP P R) //\\ (catOP Q R).
+Proof. apply landR. apply catOP_entails_m. apply landL1. reflexivity. reflexivity.
+                    apply catOP_entails_m. apply landL2. reflexivity. reflexivity.
+Qed.
+
+Lemma catOP_land P Q R : catOP P (Q//\\R) |-- (catOP P Q) //\\ (catOP P R).
+Proof. apply landR. apply catOP_entails_m. reflexivity. apply landL1. reflexivity. 
+                    apply catOP_entails_m. reflexivity. apply landL2. reflexivity.
+Qed.
