src/SPredTotal.v
@@ -1,0 +1,53 @@
+(*===========================================================================
+   Embedding of total states (ProcState) into partial states (PState)
+   and associate lemmas regarding SPreds
+  ===========================================================================*)
+Require Import ssreflect ssrfun ssrbool ssrnat eqtype tuple seq fintype.
+Require Import bitsrep bitsprops bitsops bitsopsprops procstate procstatemonad pmapprops.
+Require Import monad monadinst reader SPred septac pointsto pfun cursor writer.
+
+Set Implicit Arguments.
+Unset Strict Implicit.
+Import Prenex Implicits.
+
+Transparent ILFun_Ops.
+
+(* A full machine state can be interpreted as a partial state *)
+Definition toPState (s:ProcState) : PState :=
+  fun f:Frag =>
+  match f return fragDom f -> option (fragTgt f) with
+  | Registers => fun r => Some (registers s r)
+  | Flags => fun f => Some (flags s f)
+  | Memory => fun p => Some (memory s p)
+  end. 
+
+Coercion toPState : ProcState >-> PState.
+
+Lemma totalProcState (s: ProcState) : isTotalPState s.
+Proof. move => f x. destruct f; destruct x => //.  Qed. 
+
+Require Import FunctionalExtensionality CSetoid.
+Lemma toPState_inj s1 s2 : toPState s1 === toPState s2 -> s1 = s2. 
+Proof. move => H. 
+destruct s1 as [s1r s1f s1m]. 
+destruct s2 as [s2r s2f s2m].
+unfold "===", toPState in H.
+simpl in H. 
+Admitted.
+
+Lemma eqPredProcState_sepSP (s: ProcState) R :
+  eq_pred s ** R |-- eq_pred s. 
+Proof. rewrite (eqPredTotal_sepSP_trueR _); last by apply totalProcState. by ssimpl. Qed. 
+
+Definition isClosed (P: SPred) :=
+  forall s s', stateIncludedIn s s' -> P s -> P s'.
+
+Lemma isClosed_sepSP_ltrue P:
+  isClosed P -> P ** ltrue -|- P.
+Proof.
+  move=> HClosed. split.
+  - move=> s [s1 [s2 [Hs [HPs _]]]]. eapply HClosed; [|eassumption].
+    edestruct stateSplitsAsIncludes; [eapply Hs | assumption].
+  - rewrite <-empSPR at 1. cancel2.
+Qed.
+
