src/obs.v
@@ -1,0 +1,78 @@
+(*===========================================================================
+    obs specification    
+  ===========================================================================*)
+Require Import ssreflect ssrbool ssrfun ssrnat eqtype tuple seq fintype.
+Require Import bitsrep procstate procstatemonad SPred SPredTotal septac spec.
+Require Import ioaction step bilogic OPred.
+Require Import safe.
+
+Set Implicit Arguments.
+Unset Strict Implicit.
+Import Prenex Implicits.
+
+Require Import Setoid RelationClasses Morphisms.
+Local Obligation Tactic := idtac.
+
+Program Definition obs (O: OPred) := mkspec (fun k P =>
+    forall (s: ProcState), (P ** ltrue) s -> exists o1 o2, preObs o1 o2 /\ O o2 /\ runsForWith k s o1) _ _.
+Next Obligation. move=> O k P Hsafe s Hs. 
+destruct (Hsafe _ Hs) as [o1 [o2 [PRE [OH RUNS]]]]. 
+have LE: k <= k.+1 by done.
+destruct (runsForWithLe LE RUNS) as [o' [PRE' RUNS']]. 
+exists o', o2. split => //. by rewrite -> PRE'. Qed.
+Next Obligation. move=> O k P P' [R HR] Hsafe s Hs. 
+  apply Hsafe.
+  rewrite ->lentails_eq in Hs. rewrite <-HR in Hs.
+  apply lentails_eq. rewrite ->Hs. by ssimpl.
+Qed.
+
+Local Transparent ILFun_Ops ILPre_Ops.
+
+
+(* Morphism for obs *)
+Instance obs_entails_m: Proper (lentails ==> lentails) obs.
+Proof.
+move => O O' HO. move => k R. 
+move => H1 s H2.  
+specialize (H1 s H2). 
+destruct H1 as [o1 [o2 [H3 [H4 H5]]]]. 
+exists o1, o2. split => //. split => //. 
+by apply: HO. 
+Qed. 
+
+Instance obs_equiv_m: Proper (lequiv ==> lequiv) obs.
+Proof.
+move => O O' HO. split. by rewrite HO. by rewrite <-HO. 
+Qed. 
+
+
+Lemma safeAsObs : safe -|- obs ltrue. 
+Proof. 
+apply spec_equiv => k R. 
+rewrite /safe/obs/mkspec/spec_fun/=.  
+rewrite /runsFor/runsForWith. split => H1 s H2.
+specialize (H1 _ H2). 
+destruct H1 as [s' [o STEPS]]. 
+exists o, o. split. reflexivity. split => //. by exists s'. 
+specialize (H1 _ H2). 
+destruct H1 as [o1 [o2 [H1 [_ [s' STEPS]]]]]. 
+by exists s', o1. 
+Qed. 
+
+Instance AtEx_obs O: AtEx (obs O).
+Proof.
+  move=> A f. 
+  move=> k P Hf.
+  move=> s Hs.
+  sdestruct: Hs => a Hs.
+  eapply Hf; eassumption.
+Qed.
+
+Instance AtContra_obs O: AtContra (obs O).
+Proof.
+  move=> R R' HR. move=> k P HP.
+  move=> s Hs. apply HP.
+  rewrite lentails_eq. rewrite <-HR. by rewrite -lentails_eq.
+Qed.
+
+
